theories/aneris_lang/lifting_pure.v
@@ -2,10 +2,12 @@ From iris.algebra Require Import auth gmap frac agree coPset gset frac_auth ofe.
 From iris.base_logic Require Export own gen_heap.
 From iris.bi.lib Require Import fractional.
 From iris.base_logic.lib Require Import viewshifts saved_prop gen_heap.
-From iris.program_logic Require Export weakestpre.
+From iris.program_logic Require Import weakestpre.
 From iris.program_logic Require Import ectx_lifting total_ectx_lifting.
 From iris.proofmode Require Import tactics.
-From aneris.aneris_lang Require Export helpers lang notation tactics network resources_lemmas.
+From aneris.aneris_lang Require Import
+     aneris_lang ground_lang helpers lang notation tactics
+     network resources_lemmas.
 From stdpp Require Import fin_maps gmap.
 From RecordUpdate Require Import RecordSet.
 Set Default Proof Using "Type".
@@ -22,7 +24,7 @@ lemmas. *)
 Ltac inv_head_step :=
   repeat match goal with
   | _ => progress simplify_map_eq/= (* simplify memory stuff *)
-  | H : to_val _ = Some _ |- _ => apply to_base_val in H
+  | H : aneris_to_val _ = Some _ |- _ => apply to_base_aneris_val in H
   | H : ground_lang.head_step ?e _ _ _ _ _ |- _ =>
      try (is_var e; fail 1); (* inversion yields many goals if [e] is a variable
      and can thus better be avoided. *)
@@ -35,43 +37,74 @@ Ltac inv_head_step :=
      inversion H; subst; clear H
   end.
 
-Instance into_val_val n v : IntoVal ⟨n;Val v⟩ 〈n;v〉.
+Instance into_val_val n v : IntoVal (mkExpr n (Val v)) (mkVal n v).
 Proof. done. Qed.
-Instance as_val_val n v : AsVal ⟨n;Val v⟩.
-Proof. by exists 〈n;v〉. Qed.
+Instance as_val_val n v : AsVal (mkExpr n (Val v)).
+Proof. by exists (mkVal n v). Qed.
+
+Instance into_val_ground_val v : IntoVal (Val v) v.
+Proof. done. Qed.
+Instance as_val_ground_val v : AsVal (Val v).
+Proof. by exists v. Qed.
 
 Local Ltac solve_atomic :=
   apply strongly_atomic_atomic, ectx_language_atomic;
     [inversion 1; inv_head_step; naive_solver
     |apply ectxi_language_sub_redexes_are_values; intros [] **; inv_head_step;
-       rewrite /to_val /is_Some /=; eexists; by
+       rewrite /aneris_to_val /is_Some /=; eexists; by
          match goal with
          | H: _ = _ |- _ => rewrite -H
          end
     ].
 
-Instance binop_atomic n s op v1 v2 : Atomic s ⟨n;BinOp op (Val v1) (Val v2)⟩.
+Lemma aneris_ground_fill K ip e :
+  mkExpr ip (fill (Λ := ground_ectxi_lang) K e) =
+  fill (Λ := aneris_ectxi_lang) K (mkExpr ip e).
+Proof.
+  revert e; induction K as [|k K IHK] using rev_ind; first done.
+  intros e.
+  rewrite !fill_app /= -IHK /=; done.
+Qed.
+
+Instance aneris_pure_exec_fill
+         (K : list ectx_item) ip (φ : Prop) (n : nat) (e1 e2 : expr) :
+  PureExec φ n (mkExpr ip e1) (mkExpr ip e2) →
+  @PureExec aneris_lang φ n
+            (mkExpr ip (@fill ground_ectxi_lang K e1))
+            (mkExpr ip (@fill ground_ectxi_lang K e2)).
+Proof.
+  intros.
+  rewrite !aneris_ground_fill.
+  eapply pure_exec_ctx; first apply _; done.
+Qed.
+
+Instance binop_atomic n s op v1 v2 :
+  Atomic s (mkExpr n (BinOp op (Val v1) (Val v2))).
 Proof. solve_atomic. Qed.
-Instance alloc_atomic n s v : Atomic s ⟨n;Alloc (Val v)⟩.
+Instance alloc_atomic n s v : Atomic s (mkExpr n (Alloc (Val v))).
 Proof. solve_atomic. Qed.
-Instance load_atomic n s v : Atomic s ⟨n;Load (Val v)⟩.
+Instance load_atomic n s v : Atomic s (mkExpr n (Load (Val v))).
 Proof. solve_atomic. Qed.
-Instance store_atomic n s v1 v2 : Atomic s ⟨n;Store (Val v1) (Val v2)⟩.
+Instance store_atomic n s v1 v2 : Atomic s (mkExpr n (Store (Val v1) (Val v2))).
 Proof. solve_atomic. Qed.
-Instance cmpxchg_atomic n s v0 v1 v2 : Atomic s ⟨n;CAS (Val v0) (Val v1) (Val v2)⟩.
+Instance cmpxchg_atomic n s v0 v1 v2 :
+  Atomic s (mkExpr n (CAS (Val v0) (Val v1) (Val v2))).
 Proof. solve_atomic. Qed.
-Instance fork_atomic n s e : Atomic s ⟨n;Fork e⟩.
+Instance fork_atomic n s e : Atomic s (mkExpr n (Fork e)).
 Proof. solve_atomic. Qed.
-Instance skip_atomic n s : Atomic s ⟨n;Skip⟩.
+Instance skip_atomic n s : Atomic s (mkExpr n Skip).
 Proof. solve_atomic. Qed.
 
-Instance newsocket_atomic n v0 v1 v2 s : Atomic s ⟨n; NewSocket (Val v0) (Val v1) (Val v2)⟩.
+Instance newsocket_atomic n v0 v1 v2 s :
+  Atomic s (mkExpr n  (NewSocket (Val v0) (Val v1) (Val v2))).
 Proof. solve_atomic. Qed.
-Instance socketbind_atomic n v0 v1  s : Atomic s ⟨n; SocketBind (Val v0) (Val v1)⟩.
+Instance socketbind_atomic n v0 v1  s :
+  Atomic s (mkExpr n (SocketBind (Val v0) (Val v1))).
 Proof. solve_atomic. Qed.
-Instance sendto_atomic n v0 v1 v2 s : Atomic s ⟨n; SendTo (Val v0) (Val v1) (Val v2)⟩.
+Instance sendto_atomic n v0 v1 v2 s :
+  Atomic s (mkExpr n (SendTo (Val v0) (Val v1) (Val v2))).
 Proof. solve_atomic. Qed.
-Instance receivefrom_atomic n v s : Atomic s ⟨n; ReceiveFrom (Val v)⟩.
+Instance receivefrom_atomic n v s : Atomic s (mkExpr n (ReceiveFrom (Val v))).
 Proof. solve_atomic. Qed.
 
 Local Ltac solve_exec_safe :=
@@ -85,8 +118,8 @@ Local Ltac solve_exec_puredet :=
   simpl; intros; inv_head_step;
   first (by repeat match goal with
                    | H: _ ∧ _ |- _ => destruct H as [??]; simplify_eq
-                   | H : ground_lang.to_val _ = Some _ |- _ =>
-                     rewrite ground_lang.to_of_val in H; simplify_eq
+                   | H : to_val _ = Some _ |- _ =>
+                     rewrite to_of_val in H; simplify_eq
                    end);
   try by match goal with
          | H : socket_step _ _ _ _ _ _ _ _ _ |- _ =>
@@ -96,81 +129,87 @@ Local Ltac solve_pure_exec :=
   simplify_eq; rewrite /PureExec; intros; apply nsteps_once, pure_head_step_pure_step;
     constructor; [solve_exec_safe | solve_exec_puredet].
 
-Class AsRecV (v : ground_lang.val) (f x : binder) (erec : ground_lang.expr) :=
+Class AsRecV (v : val) (f x : binder) (erec : expr) :=
   as_recv : v = RecV f x erec.
 Hint Mode AsRecV ! - - - : typeclass_instances.
 Definition AsRecV_recv f x e : AsRecV (RecV f x e) f x e := eq_refl.
 Hint Extern 0 (AsRecV (RecV _ _ _) _ _ _) =>
   apply AsRecV_recv : typeclass_instances.
 
-Instance pure_rec f x (erec : ground_lang.expr) :
-  PureExec True 1 ⟨n;Rec f x erec⟩ ⟨n;Val $ RecV f x erec⟩.
+Instance pure_rec f x (erec : expr) :
+  PureExec True 1 (mkExpr n (Rec f x erec)) (mkExpr n (Val $ RecV f x erec)).
 Proof. solve_pure_exec. Qed.
-Instance pure_pairc (v1 v2 : ground_lang.val) :
-  PureExec True 1 ⟨n;(Pair (Val v1) (Val v2))⟩ ⟨n;(Val $ PairV v1 v2)⟩.
+Instance pure_pairc (v1 v2 : val) :
+  PureExec True 1 (mkExpr n (Pair (Val v1) (Val v2))) (mkExpr n (Val $ PairV v1 v2)).
 Proof. solve_pure_exec. Qed.
-Instance pure_injlc (v : ground_lang.val) :
-  PureExec True 1 ⟨n;(InjL $ Val v)⟩ ⟨n;(Val $ InjLV v)⟩.
+Instance pure_injlc (v : val) :
+  PureExec True 1 (mkExpr n (InjL $ Val v)) (mkExpr n (Val $ InjLV v)).
 Proof. solve_pure_exec. Qed.
-Instance pure_injrc (v : ground_lang.val) :
-  PureExec True 1 ⟨n;(InjR $ Val v)⟩ ⟨n;(Val $ InjRV v)⟩.
+Instance pure_injrc (v : val) :
+  PureExec True 1 (mkExpr n (InjR $ Val v)) (mkExpr n (Val $ InjRV v)).
 Proof. solve_pure_exec. Qed.
 
-Instance pure_beta f x erec (v1 v2 : ground_lang.val) `{!AsRecV v1 f x erec} :
-  PureExec True 1 ⟨n;(App (Val v1) (Val v2))⟩ ⟨n;(subst' x v2 (subst' f v1 erec))⟩.
+Instance pure_beta f x erec (v1 v2 : val) `{!AsRecV v1 f x erec} :
+  PureExec True 1 (mkExpr n (App (Val v1) (Val v2)))
+           (mkExpr n (subst' x v2 (subst' f v1 erec))).
 Proof. unfold AsRecV in *. solve_pure_exec. Qed.
 
 Instance pure_unop op v v' :
-  PureExec (un_op_eval op v = Some v') 1 ⟨n;UnOp op (Val v)⟩ ⟨n;ground_lang.of_val v'⟩.
+  PureExec (un_op_eval op v = Some v') 1 (mkExpr n (UnOp op (Val v)))
+           (mkExpr n (of_val v')).
 Proof. solve_pure_exec. Qed.
 
 Instance pure_binop op v1 v2 v' :
   PureExec (bin_op_eval op v1 v2 = Some v') 1
-           ⟨n;BinOp op (Val v1) (Val v2)⟩ ⟨n;ground_lang.of_val v'⟩.
+           (mkExpr n (BinOp op (Val v1) (Val v2))) (mkExpr n (of_val v')).
 Proof. solve_pure_exec. Qed.
 
-Instance pure_if_true e1 e2 : PureExec True 1 ⟨n;If (Val $ LitV $ LitBool true) e1 e2⟩ ⟨n;e1⟩.
+Instance pure_if_true e1 e2 :
+  PureExec True 1 (mkExpr n (If (Val $ LitV $ LitBool true) e1 e2)) (mkExpr n e1).
 Proof. solve_pure_exec. Qed.
 
-Instance pure_if_false e1 e2 : PureExec True 1 ⟨n;If (Val $ LitV $ LitBool false) e1 e2⟩ ⟨n;e2⟩.
+Instance pure_if_false e1 e2 :
+  PureExec True 1 (mkExpr n (If (Val $ LitV $ LitBool false) e1 e2))
+           (mkExpr n e2).
 Proof. solve_pure_exec. Qed.
 
 Instance pure_fst v1 v2  :
-  PureExec True 1 ⟨n;Fst (PairV v1 v2)⟩ ⟨n;Val v1⟩.
+  PureExec True 1 (mkExpr n (Fst (PairV v1 v2))) (mkExpr n (Val v1)).
 Proof. solve_pure_exec. Qed.
 
 Instance pure_snd v1 v2  :
-  PureExec True 1 ⟨n;Snd (PairV v1 v2)⟩ ⟨n;Val v2⟩.
+  PureExec True 1 (mkExpr n (Snd (PairV v1 v2))) (mkExpr n (Val v2)).
 Proof. solve_pure_exec. Qed.
 
 Instance pure_find_from v0 v1 n1 v2 v' :
   PureExec (index n1 v2 v0 = v' ∧ Z.of_nat n1 = v1) 1
-           ⟨n;FindFrom (Val $ LitV $ LitString v0)
+           (mkExpr n (FindFrom (Val $ LitV $ LitString v0)
                        (Val $ LitV $ LitInt v1)
-                       (Val $ LitV $ LitString v2)⟩
-           ⟨n;ground_lang.of_val (option_nat_to_val v')⟩.
+                       (Val $ LitV $ LitString v2)))
+           (mkExpr n (ground_lang.of_val (option_nat_to_val v'))).
 Proof. solve_pure_exec. Qed.
 
 Instance pure_substring v0 v1 n1 v2 n2 v' :
   PureExec (substring n1 n2 v0 = v' ∧ Z.of_nat n1 = v1 ∧ Z.of_nat n2 = v2) 1
-           ⟨n;Substring (LitV $ LitString v0) (LitV $ LitInt v1) (LitV $ LitInt v2)⟩
-           ⟨n;ground_lang.of_val (LitV $ LitString v')⟩.
+           (mkExpr
+              n (Substring
+                   (LitV $ LitString v0) (LitV $ LitInt v1) (LitV $ LitInt v2)))
+           (mkExpr n (ground_lang.of_val (LitV $ LitString v'))).
 Proof. solve_pure_exec. Qed.
 
 Instance pure_case_inl v e1 e2  :
-  PureExec True 1 ⟨n;Case (Val $ InjLV v) e1 e2⟩ ⟨n;App e1 (Val v)⟩.
+  PureExec True 1 (mkExpr n (Case (Val $ InjLV v) e1 e2))
+           (mkExpr n (App e1 (Val v))).
 Proof. solve_pure_exec. Qed.
 
 Instance pure_case_inr v e1 e2 :
-  PureExec True 1 ⟨n;Case (Val $ InjRV v) e1 e2⟩ ⟨n;App e2 (Val v)⟩.
+  PureExec True 1 (mkExpr n (Case (Val $ InjRV v) e1 e2))
+           (mkExpr n (App e2 (Val v))).
 Proof. solve_pure_exec. Qed.
 
 Instance pure_make_address v1 v2 :
   PureExec True 1
-           ⟨n;MakeAddress (LitV (LitString v1)) (LitV (LitInt (v2)))⟩
-           ⟨n;LitV (LitSocketAddress (SocketAddressInet v1 (Z.to_pos v2)))⟩.
+           (mkExpr n (MakeAddress (LitV (LitString v1)) (LitV (LitInt (v2)))))
+           (mkExpr
+              n (LitV (LitSocketAddress (SocketAddressInet v1 (Z.to_pos v2))))).
 Proof. solve_pure_exec. Qed.
-
-Local Hint Constructors head_step : core.
-Local Hint Resolve alloc_fresh : core.
-Local Hint Resolve to_of_val : core.
