theories/aneris_lang/aneris_lang.v
@@ -1,0 +1,5 @@
+From aneris.aneris_lang Require Export lang.
+
+Canonical Structure aneris_ectxi_lang := EctxiLanguage aneris_lang_mixin.
+Canonical Structure aneris_ectx_lang := EctxLanguageOfEctxi aneris_ectxi_lang.
+Canonical Structure aneris_lang := LanguageOfEctx aneris_ectx_lang.
