theories/aneris_lang/ground_lang.v
@@ -1,0 +1,5 @@
+From aneris.aneris_lang Require Export lang.
+
+Canonical Structure ground_ectxi_lang := EctxiLanguage base_mixin.
+Canonical Structure ground_ectx_lang := EctxLanguageOfEctxi ground_ectxi_lang.
+Canonical Structure ground_lang := LanguageOfEctx ground_ectx_lang.
