theories/aneris_lang/lib/network_helpers.v
@@ -1,6 +1,6 @@
 From iris.program_logic Require Export weakestpre.
 From iris.proofmode Require Import tactics.
-From aneris.aneris_lang Require Import lang lifting tactics proofmode notation.
+From aneris.aneris_lang Require Import lang tactics proofmode notation.
 From aneris.aneris_lang.lib Require Import assert.
 
 Section code.
@@ -42,55 +42,54 @@ Import uPred.
 Section library.
   Context `{dG : distG Σ}.
 
-  Lemma unSOME_spec n v v' :
-    {{{ ⌜v = SOMEV v'⌝ }}}
-      ⟨n;unSOME (Val v)⟩
-    {{{ RET 〈n;v'〉; True }}}.
+  Lemma unSOME_spec ip v v' :
+    {{{ ⌜v = SOMEV v'⌝ }}} unSOME (Val v) @[ip] {{{ RET v'; True }}}.
   Proof.
     iIntros (Φ ->) "HΦ".
     wp_lam. wp_match. by iApply "HΦ".
   Qed.
 
-  Lemma listen_spec P Q h s R T a handler φ:
-    let n := ip_of_address a in
+  Lemma listen_spec ip P Q h s R T a handler φ:
+    ip = ip_of_address a →
     saddress s = Some a →
     (∀ m,
       {{{ ⌜m_destination m = a⌝ ∗ P ∗
-          ((⌜m ∉ R⌝ ∗ h s↦[n]{1/2} (s, {[m]} ∪ R, T) ∗ φ m) ∨
-          (⌜m ∈ R⌝ ∗ h s↦[n]{1/2} (s, R, T)))
+          ((⌜m ∉ R⌝ ∗ h s↦[ip]{1/2} (s, {[m]} ∪ R, T) ∗ φ m) ∨
+          (⌜m ∈ R⌝ ∗ h s↦[ip]{1/2} (s, R, T)))
       }}}
-         ⟨n; (Val handler) #(m_body m) #(m_sender m)⟩
-      {{{ v, RET 〈n;v〉; Q v }}}) -∗
-      {{{ P ∗ h s↦[n]{1/2} (s, R, T) ∗ a ⤇ φ }}}
-         ⟨ n; listen #(LitSocket h) (Val handler) ⟩
-      {{{ v, RET 〈n;v〉; Q v }}}.
+         (Val handler) #(m_body m) #(m_sender m) @[ip]
+      {{{ v, RET v; Q v }}}) -∗
+      {{{ P ∗ h s↦[ip]{1/2} (s, R, T) ∗ a ⤇ φ }}}
+         listen #(LitSocket h) (Val handler) @[ip]
+      {{{ v, RET v; Q v }}}.
   Proof.
      iIntros (n Haddr) "#Hhandler". iLöb as "IH".
      iAlways. iIntros (Φ) "(HP & Hsocket & #Hsi) HΦ".
      wp_rec. wp_let. rewrite /n. wp_bind (ReceiveFrom _).
-     wp_apply (wp_receive_from_2 with "[$]"); first done.
+     wp_apply (aneris_wp_receive_from_2 with "[$]"); [done|done|].
      iIntros (r) "[(-> & Hs) | Hrd ]"; simpl.
      - wp_pures. iApply ("IH" with "[-HΦ]"); by iFrame.
-     - iDestruct "Hrd" as (m Hdst ->) "[ (% & Hs & _ & Hφ) | (% & Hs) ]"; wp_pures;
+     - iDestruct "Hrd" as (m Hdst ->) "[ (% & Hs & Hφ) | (% & Hs) ]"; wp_pures;
          wp_apply ("Hhandler" with "[-HΦ] [HΦ]"); eauto with iFrame.
   Qed.
 
-  Lemma listen_wait_spec h s R T a φ :
-    let n := ip_of_address a in
+  Lemma listen_wait_spec ip h s R T a φ :
+    ip = ip_of_address a →
     saddress s = Some a →
-  {{{ h s↦[n]{1/2} (s, R, T) ∗ a ⤇ φ}}}
-     ⟨ n; listen_wait #(LitSocket h) ⟩
-  {{{ m, RET 〈n;(#(m_body m), #(m_sender m))〉;
-      ((⌜m ∉ R⌝ ∗ h s↦[n]{1/2} (s, {[ m ]} ∪ R, T) ∗ a ⤇ φ ∗ ▷ φ m) ∨
-       ⌜m ∈ R⌝ ∗ h s↦[n]{1/2} (s, R, T))
+  {{{ h s↦[ip]{1/2} (s, R, T) ∗ a ⤇ φ}}}
+     listen_wait #(LitSocket h) @[ip]
+  {{{ m, RET (#(m_body m), #(m_sender m));
+      ((⌜m ∉ R⌝ ∗ h s↦[ip]{1/2} (s, {[ m ]} ∪ R, T) ∗ a ⤇ φ ∗ ▷ φ m) ∨
+       ⌜m ∈ R⌝ ∗ h s↦[ip]{1/2} (s, R, T))
   }}}.
   Proof.
     iIntros (n Haddr Φ) "(Hs & #Hsi) HΦ".
     iLöb as "IH". wp_rec.
-    wp_apply (wp_receive_from_2 with "[$Hs]"); first done; try iFrame "#".
+    wp_apply (aneris_wp_receive_from_2 with "[$Hs]");
+      [done|done|by iFrame "#"|].
     iIntros (r)  "[(-> & Hs) | Hrd ]"; simpl; wp_pures.
     - by iApply ("IH" with "Hs HΦ").
-    - iDestruct "Hrd" as (m Hdst ->) "[ (% & Hs & _ & Hφ) | (% & Hs) ]"; wp_pures.
+    - iDestruct "Hrd" as (m Hdst ->) "[ (% & Hs & Hφ) | (% & Hs) ]"; wp_pures.
       + iApply "HΦ". iLeft. eauto with iFrame.
       + iApply "HΦ". iRight. eauto with iFrame.
   Qed.
